Reorganize some files

ref_impl/src/verifier/experiments/fstar_experiments/project/bosqueTypes.fst
@@ -5,17 +5,16 @@ open BosqueTerms
 
 // Convention with UnionTerm: 
 // its elements should be unique
-noeq type bosqueType =
-| BTypeError 
+type bosqueType =
 | BTypeNone
 | BTypeInt
 | BTypeBool
 | BTypeUnion : bosqueType -> bosqueType -> bosqueType
+// The bool indicates if the Empty Tuple is open or not
+| BTypeEmptyTuple : bool -> bosqueType
 // The bool indicates if the Tuple is open or not
-| BTypeEmptyTuple
 | BTypeTuple : bool -> n:nat -> sequence bosqueType n -> bosqueType
-// | BTypeTuple : bool -> n:nat -> sequence bosqueTerm n -> bosqueType
-
+| BTypeError 
 
 (* --------------------------------------------------------------- *)
 (* Operations on Bosque Types *)
@@ -23,37 +22,43 @@ noeq type bosqueType =
 (* Definition of equality relation on Bosque types *)
 val eqType : bosqueType -> bosqueType -> bool
 let eqType x y = match x, y with
-| BTypeError, BTypeError -> true 
 | BTypeNone, BTypeNone -> true
 | BTypeInt, BTypeInt -> true
 | BTypeBool, BTypeBool -> true
 | BTypeUnion _ _ , BTypeUnion _ _ -> true    // FIX: This is incomplete
+| BTypeEmptyTuple b1, BTypeEmptyTuple b2 -> b1 = b2
 | BTypeTuple _ _ _, BTypeTuple _ _ _ -> true // FIX: This is incomplete
-| _, _ -> false 
+| BTypeError, BTypeError -> true 
+| _, _ -> false
 
-val mapTermToType : #n:nat -> (x: sequence bosqueTerm n) -> Tot (sequence bosqueType n) (decreases x)
+(* Definition of getType *)
+val getType_aux : #n:nat -> (x: sequence bosqueTerm n) -> Tot (sequence bosqueType n) (decreases x)
 val getType : x:bosqueTerm -> Tot bosqueType (decreases x)
 let rec getType x = match x with
 | BError -> BTypeError
 | BNone -> BTypeNone
 | BInt _ -> BTypeInt
 | BBool _ -> BTypeBool
-| BTuple n y -> BTypeTuple false n (mapTermToType y)
-and mapTermToType #n x1 = match x1 with
+| BTuple n CNil -> if (n <> 0) then BTypeError else BTypeEmptyTuple false 
+| BTuple n (CCons y ys) -> BTypeTuple false n (getType_aux #n (CCons y ys))
+and 
+getType_aux #n x = match x with
 | CNil -> CNil
-| CCons y1 ys1 -> CCons (getType y1) (mapTermToType ys1)
+| CCons y ys -> CCons (getType y) (getType_aux ys)
 
+(* Definition to encode the subtype relation on Bosque types *)
 // forall x y . bosqueSubtypeOf x y <===> x :> y
 val bosqueSubtypeOf : bosqueType -> bosqueType -> (Tot bool)
 let rec bosqueSubtypeOf x y = match x, y with
-| BTypeError, BTypeError -> true
 | BTypeNone, BTypeNone -> true
 | BTypeInt, BTypeInt -> true
 | BTypeBool, BTypeBool -> true
 | BTypeUnion x1 y1, BTypeUnion x2 y2 -> (bosqueSubtypeOf x1 x2 || bosqueSubtypeOf y1 x2) 
   && (bosqueSubtypeOf x1 y2 || bosqueSubtypeOf y1 y2)
 | BTypeUnion x1 y1, z -> bosqueSubtypeOf x1 z || bosqueSubtypeOf y1 z 
+| BTypeEmptyTuple b1, BTypeEmptyTuple _ -> b1
 // Missing case: BTuple
+| BTypeError, BTypeError -> true
 | _, _ -> false
 
 (* ---------------------------------------------------------------- *)
